kuiops/common/tc2d_to/Kuiops.Kernel.GEMM.TensorCore2D.To.EpilogueState.fsti
@@ -109,6 +109,21 @@ let epilogue_warp_input
     ((tid / warp_size) / (bn / (wn * tn)))
     ((tid / warp_size) % (bn / (wn * tn)))
 
+(* Keep this folded in call-site specifications: expanding the nested
+   chest operations makes F*'s core typechecker spend minutes comparing them. *)
+let epilogue_warp_output
+  (#m #n : nat)
+  (comb_r : binop real)
+  (rC : chest2 real m n)
+  (bm bn tm tn wm wn : pos)
+  (#_ : squash (bm /?+ m /\ bn /?+ n /\
+                wm * tm /?+ bm /\ wn * tn /?+ bn))
+  (bid : natlt (m / bm * (n / bn)))
+  (tid : natlt (bm / (wm * tm) * (bn / (wn * tn)) * warp_size))
+  (rAcc : chest2 real (wm * tm) (wn * tn))
+  : chest2 real (wm * tm) (wn * tn)
+= chest_comb comb_r (epilogue_warp_input rC bm bn tm tn wm wn bid tid) rAcc
+
 let output_fragment_post
   (#et : Type0) {| scalar et, real_like et, has_vec_cpy et |}
   (#m #n : nat)
